theories/program_logic/delay_examples.v
@@ -1,0 +1,121 @@
+
+From iris.proofmode Require Import base tactics classes.
+From iris.base_logic.lib Require Export fancy_updates.
+From shiris.program_logic Require Import delaystate.
+From shiris.program_logic Require Import delaywp.
+
+(*Example programs *)
+Definition fib' (st: nat * nat * nat): delay ((nat * nat * nat) + nat).
+refine (match st with
+|(0, x, y) => Answer $ inr $ x
+|((S n), x, y) => Answer $ inl (n, y, x + y)
+end).
+Defined.
+
+Definition fib (n: nat): delay nat := delaystate.iter fib' (n, 0, 1).
+
+Lemma test_fib: (λ n, ev_delay 10 (fib n)) <$> [0; 1; 2; 3; 4; 5; 6; 7] = Some <$> [0; 1; 1; 2; 3; 5; 8; 13].
+Proof.
+  reflexivity.
+Qed.
+
+Fixpoint coq_fib (n1 n2: nat) (n: nat): nat :=
+    match n with
+    |O => n1
+    |S n' => match n' with
+             | O => n2 
+             | S n'' => coq_fib n1 n2 n' + coq_fib n1 n2 n''
+             end
+    end.
+
+Section state_ad.
+Context `{! inG Σ (heapR natO)}.
+
+Lemma post' (n1 n2 n: nat) (ret: nat): iProp Σ.
+refine( ⌜ret = coq_fib n1 n2 n⌝%I).
+Defined.
+
+Locate "+".
+Lemma post'' (n1 n2 n: nat) (res: (nat * nat * nat) + nat): iProp Σ.
+refine (match n with
+        |O    => ⌜res = inr n1⌝
+        |S n' => ⌜res = inl (n', n2, Nat.add n1 n2)⌝ 
+end)%I.
+Defined.
+
+(* one execution of fib either returns the addition and takes one from n
+   or n is zero and returns the answer 
+*)
+Lemma verify_fib' n1 n2 n: 
+    True -∗ wp_delay (fib' (n, n1, n2)) (post'' n1 n2 n).
+Proof.
+    iIntros "_".
+    unfold fib'. unfold post''.
+    destruct n.
+    - by iApply wp_delay_return.
+    - by iApply wp_delay_return.
+Qed.
+
+(* If i pick a particular n I can just unroll the loop n times*)
+Lemma verify_delay_fib_brute:
+    True -∗ @wp_delay Σ _ (fib 4) (λ ret, ⌜ret = 3⌝).
+Proof.
+    iIntros "_".
+    unfold fib.
+    iApply wp_delay_iter. 
+    iApply wp_delay_return.
+    iApply wp_delay_iter.
+    iApply wp_delay_return.
+    iApply wp_delay_iter.
+    iApply wp_delay_return.
+    iApply wp_delay_iter.
+    iApply wp_delay_return.
+    iApply wp_delay_iter.
+    iApply wp_delay_return.
+    done.
+Qed.
+
+(* To get lob induction to work I need the numbers that are passed
+    between loop states to vary. but then my post condition does
+    not always hold that needs to be generalized too.
+*)
+Lemma verify_delay_fib' n1 n2 n:
+    True -∗ wp_delay (delaystate.iter fib' (n, n1, n2)) (post' n1 n2 n).
+Proof.
+    iIntros "_".
+    (*How do i vary the IH here properly *)
+    iLöb as "IH" forall (n n1 n2).
+    unfold fib.
+    iApply wp_delay_iter. 
+    destruct n eqn: E.
+    - iApply wp_delay_return. done.
+    - iApply wp_delay_return. simpl. 
+      iNext. iDestruct ("IH" $! n0 n2) as "IH'".
+Qed.
+
+Lemma verify_delay_fib n:
+    True -∗ wp_delay (fib n) (post n).
+Proof.
+
+Definition iter_adder (l k: nat): () -> state_delay (gmap nat nat) (() + nat) :=
+  λ _, x  ← get l ;
+       y  ← get k ; 
+       if x =? 0 then mret $ inr y 
+       else put l (x - 1) ;; put k (y + 1) ;; mret $ inl () .
+
+Definition fib_state' (l1 l2: nat) (n: nat): state_delay (gmap nat nat) (nat + nat) :=
+    match n with
+    | S n' => n1 ← get l1 ;
+              n2 ← get l2 ;
+              put l1 n1 ;; put l2 (n1 + n2) ;; mret $ inl n'
+    | O => inr <$> get l2
+    end.
+
+Definition fib_state (l1 l2 n: nat): state_delay (gmap nat nat) nat := 
+    iter_state_delay (fib_state' l1 l2) n.
+
+Lemma verify_delay_state_fib l1 l2 n:
+    ∀ γ, points_to γ l1 1 ∗ points_to γ l2 1 -∗
+            wp (state_interp γ) (fib_state l1 l2 n) (λ ret, ⌜ret = coq_fib 0 1 n⌝).
+Proof.
+Admitted.
